


\begin{eqnarray*}
r_1 & = & [ k_1 \times  E \times  S ]\\%
r_{-1} & = & [ k_{-1} \times  \hbox{\textit{E:S}} ]\\%
r_2 & = & [ k_2 \times  \hbox{\textit{E:S}} ]\\%
%
E & = & r_1{\downarrow} +  r_{-1}{\uparrow}  +  r_2{\uparrow} \\%
S & = & r_1{\downarrow}  +  r_{-1}{\uparrow} \\%
\hbox{\textit{E:S}} & = & r_1{\uparrow}  +  r_{-1}{\downarrow}  +  r_2{\downarrow} \\%
P & = & r_2{\uparrow} \\%
%
(E \sync{\{r_1, r_{-1}, r_2\}} (S \sync{\{r_1, r_{-1}\}} (\hbox{\textit{E:S}} \sync{\{r_2\}} P)))%
\end{eqnarray*}
